src/triple/core.v
@@ -3,13 +3,13 @@
     supports registers, flags and memory. *)
 Require Import Ssreflect.ssreflect Ssreflect.ssrfun Ssreflect.ssrbool Ssreflect.ssrnat Ssreflect.eqtype Ssreflect.tuple Ssreflect.seq Ssreflect.fintype.
 Require Import x86proved.bitsrep x86proved.bitsprops x86proved.bitsops x86proved.bitsopsprops x86proved.x86.procstate x86proved.x86.procstatemonad x86proved.pmapprops x86proved.x86.ioaction.
-Require Import x86proved.monad x86proved.monadinst x86proved.reader x86proved.spred x86proved.opred x86proved.spredtotal x86proved.septac x86proved.pointsto x86proved.pfun x86proved.cursor x86proved.writer.
+Require Import x86proved.monad x86proved.monadinst x86proved.reader x86proved.spred x86proved.spredtotal x86proved.septac x86proved.pointsto x86proved.pfun x86proved.cursor x86proved.writer.
 Require Import x86proved.common_tactics x86proved.common_definitions.
 
 Module Import tripleconfig.
   Export Ssreflect.ssreflect  Ssreflect.ssrfun Ssreflect.ssrbool (* for [==] notation *) Ssreflect.ssrnat (* for getting levels right *) Ssreflect.eqtype Ssreflect.tuple Ssreflect.seq (* for [++] *) Ssreflect.fintype.
   Export x86proved.x86.procstate (* for [ProcState] *) (*x86proved.x86.procstatemonad (* for [ST] *)*).
-  Export x86proved.spred (* for [SPred], [lentails] *) x86proved.opred (* for [OPred] *) x86proved.spredtotal (* for coercion [ProcState >-> PState] *).
+  Export x86proved.spred (* for [SPred], [lentails] *) x86proved.spredtotal (* for coercion [ProcState >-> PState] *).
   Export x86proved.monad (* for [bind] and [retn] *).
 
   Global Set Implicit Arguments.
@@ -20,38 +20,27 @@ Import Prenex Implicits.
 
 (** Hoare triple for machine state monad *)
 (** We ocassionally talk about the return value *)
-Definition valued_TRIPLE {T} (v : T) (P:SPred) (c:ST T) (O:OPred) (Q:SPred) :=
+Require Import step.
+Definition valued_TRIPLE {T} (v : T) (P:SPred) (c:ST T) (o:Actions) (Q:SPred) :=
   forall (s:ProcState), P s ->
-    exists f o, c s = (o, (f, Success _ v)) /\ O (outputToActions o) /\ Q f.
+    exists f, IOM_matches (c s) o = Some(f, Success _ v) /\ Q f. 
 Notation TRIPLE := (@valued_TRIPLE unit tt).
 
 (** The general rule for dealing with [TRIPLE] by computation *)
-Lemma triple_fin {T} (v : T) (P:SPred) (c:ST T) (O:OPred) (Q:SPred)
+Lemma triple_fin {T} (v : T) (P:SPred) (c:ST T) o (Q:SPred)
       (H : forall (s:ProcState),
              P (toPState s)
-             -> let trace := c s in
-                let outputs := fst trace in
-                let f := fst (snd trace) in
-                let ex := snd (snd trace) in
-                match ex with
-                  | Success v' => v = v' /\ O (outputToActions outputs) /\ Q (toPState f)
-                  | Error _ => False
+             -> let result := IOM_matches (c s) o in
+                match result with
+                  | Some (f, Success v') => v = v' /\ Q f
+                  | _ => False
                 end)
-: valued_TRIPLE v P c O Q.
+: valued_TRIPLE v P c o Q.
 Proof.
   move => s H'.
   specialize (H s H'); simpl in H.
-  generalize dependent (c s) => *.
-  do ![ progress subst
-      | progress destruct_head False
-      | progress destruct_head errorMT
-      | progress destruct_head OutputM
-      | progress destruct_head Result
-      | progress destruct_head prod
-      | progress destruct_head unit
-      | progress destruct_head and
-      | progress split_and
-      | by do !esplit ].
+  destruct (IOM_matches (c s) o) => //. destruct p as [f r]. 
+  destruct r => //. destruct H. subst. by exists f. 
 Qed.
 
 Ltac triple_hnf :=
