src/x86/step.v
@@ -23,42 +23,44 @@ Definition step : ST unit :=
   evalInstr instr.
 (*=End *)
 
+Fixpoint IOM_matches T (m:IOM Chan Data T) (o:Actions) : option T :=
+  match m, o with
+  | monadinst.Out ch d rest, ioaction.Out ch' d'::o' => 
+    if (ch==ch') && (d==d') then IOM_matches rest o' else None
+  | monadinst.In ch f, ioaction.In ch' d::o' => 
+    if ch==ch' then IOM_matches (f d) o' else None
+  | retnIO v, nil => Some v
+  | _, _ => None              
+  end.
+
+Lemma IOM_matches_bind o1 : forall T (m: IOM Chan Data T) U  v1 (f: T -> IOM Chan Data U) o2 v2, 
+  IOM_matches m o1 = Some v1 -> 
+  IOM_matches (f v1) o2 = Some v2 ->
+  IOM_matches (bind m f) (o1++o2) = Some v2.
+Proof. induction o1. 
+- move => T m U v1 f o2 v2. destruct m => //. move => /= [->] H. by rewrite H. 
+- move => T m U v1 f o2 v2 H1 H2. 
+  destruct m => //. destruct a => //. 
+  simpl in H1. 
+  case E: (ch==c); last by rewrite E in H1. 
+  case E': (d == d0); last by rewrite E' andbF in H1.  
+  rewrite E E'/= in H1. 
+  rewrite /= E E' /=. apply: IHo1. apply H1. apply H2. 
+- destruct a => //. 
+  simpl in H1. 
+  case E: (ch==c); last by rewrite E in H1. 
+  rewrite E/= in H1. 
+  rewrite /= E /=. apply: IHo1. apply H1. apply H2. 
+Qed.
+ 
 (* Labelled transition from s to s' with actions o *)
-Definition oneStep s o s' :=
-  exists output, o = outputToActions output /\ step s = (output, (s', Success _ tt)).
+Definition oneStep s o s' := IOM_matches (step s) o = Some (s', Success _ tt). 
 
 (* Takes k steps from s to s' with events o *)
 Fixpoint manyStep k s o s' :=
   if k is k'.+1
   then exists s'' o1 o2, o = o1 ++ o2 /\ oneStep s o1 s'' /\ manyStep k' s'' o2 s'
   else o = nil /\ s = s'.
-
-Lemma doManyStep k : forall s o s', (exists out, outputToActions out = o /\
-  doMany k step s = (out, (s', (Success _ tt)))) <-> manyStep k s o s'.
-Proof. induction k => /= s o s'.
-split. - by move => [out [<- [<- ->]]].
-- move => [H1 H2]. exists nil. by subst.
-
-case E: (step s) => [out0 [s0 x]].
-split. move => [out [H1 H2]].
-destruct x => //.
-case E': (doMany k step s0) => [s1 x'].
-rewrite E' in H2. injection H2 => [H3 H4]. subst. clear H2.
-eexists _. exists (outputToActions out0), (outputToActions s1).
-split. unfold outputToActions. by rewrite map_cat.
-split. rewrite /oneStep. exists out0. split => //. destruct x. eapply E.
-apply IHk. by exists s1.
-
-move => [s'' [o1 [o2 [H1 [[o3 [H2a H2b]] H3]]]]].
-subst. rewrite H2b in E.
-injection E => [E1 E2]. subst. clear E.
-move => <-. case E': (doMany k step s0) => [s1 x'].
-specialize (IHk s0 o2 s').
-destruct IHk as [_ IHk]. specialize (IHk H3).
-destruct IHk as [out [H1 H2]]. subst. exists (o3 ++ out).
-split. unfold outputToActions. by rewrite map_cat.
-rewrite E' in H2.  congruence.
-Qed.
 
 Lemma manyStepLe k : forall k', k' <= k ->
   forall s o s', manyStep k s o s' -> exists o' s'', preActions o' o /\ manyStep k' s o' s''.
