src/triple/monad.v
@@ -8,37 +8,34 @@ Require Import x86proved.triple.roc.
 
 Import Prenex Implicits.
 
-Lemma triple_skip P : TRIPLE P (retn tt) empOP P.
-Proof.  move => s pre; exists s, nil; intuition. done. Qed.
+Lemma triple_skip P : TRIPLE P (retn tt) nil P.
+Proof.  move => s pre; exists s; intuition. Qed.
 
-Lemma valued_triple_seqcat {A B} P P' P'' O1 O2 c1 c2 (v : A) (v' : B) O :
-  catOP O1 O2 |-- O ->
-  valued_TRIPLE v P c1 O1 P' ->
-  valued_TRIPLE v' P' (c2 v) O2 P'' ->
-  valued_TRIPLE v' P (bind c1 c2) O P''.
+Require Import monadinst step.
+Lemma valued_triple_seqcat {A B} P P' P'' o1 o2 c1 c2 (v : A) (v' : B) o :
+  o1 ++ o2 = o ->
+  valued_TRIPLE v P c1 o1 P' ->
+  valued_TRIPLE v' P' (c2 v) o2 P'' ->
+  valued_TRIPLE v' P (bind c1 c2) o P''.
 Proof.
-  move => HO T1 T2. rewrite <- HO; clear HO.
-  do !(idtac;
-       match goal with
-         | _ => move => ?
-         | _ => progress hnf in *
-         | _ => progress destruct_head_hnf ex
-         | _ => progress destruct_head_hnf and
-         | _ => progress hyp_rewrite *
-         | [ H : forall s : ProcState, ILFunFrm_pred ?P (toPState s) -> _, Ps : _ |- _ ] => specialize (H _ Ps)
-       end).
-  do !esplit; by [ eassumption | rewrite /outputToActions map_cat ].
-Qed.
+  move => HO T1 T2. rewrite <- HO; clear HO. 
+  move => s pre. 
+  elim (T1 s pre) => [s' [H pre']].
+  elim (T2 s' pre') => [s'' [H' post]].
+  exists s''. split => //.
+  by apply: (IOM_matches_bind H).
+Qed.   
 
-Lemma triple_seqcat P P' P'' O1 O2 c1 c2 O :
-  catOP O1 O2 |-- O ->
-  TRIPLE P c1 O1 P' ->
-  TRIPLE P' c2 O2 P'' ->
-  TRIPLE P (do! c1; c2) O P''.
+Lemma triple_seqcat P P' P'' o1 o2 c1 c2 o :
+  o1 ++ o2 = o ->
+  TRIPLE P c1 o1 P' ->
+  TRIPLE P' c2 o2 P'' ->
+  TRIPLE P (do! c1; c2) o P''.
 Proof. apply (valued_triple_seqcat (c2 := fun _ => c2)). Qed.
 
-Lemma triple_seq P P' P'' c1 c2 O :
-  TRIPLE P c1 empOP P' ->
-  TRIPLE P' c2 O P'' ->
-  TRIPLE P (do! c1; c2) O P''.
-Proof. move => T1 T2. apply: triple_seqcat T1 T2. by apply empOPL. Qed.
+Lemma triple_seq P P' P'' c1 c2 o :
+  TRIPLE P c1 nil P' ->
+  TRIPLE P' c2 o P'' ->
+  TRIPLE P (do! c1; c2) o P''.
+Proof. move => T1 T2. apply: triple_seqcat T1 T2. done. Qed.
+
