src/triple/roc.v
@@ -5,9 +5,9 @@ Require Import x86proved.triple.morphisms.
 
 Import Prenex Implicits.
 
-Lemma triple_roc P' Q' O' P c O Q:
-  P |-- P' -> O' |-- O -> Q' |-- Q -> TRIPLE P' c O' Q' -> TRIPLE P c O Q.
-Proof. move=> HP HO HQ H. setoid_rewrite<-HO. setoid_rewrite ->HP. by setoid_rewrite <-HQ. Qed.
+Lemma triple_roc P' Q' P c o Q:
+  P |-- P' -> Q' |-- Q -> TRIPLE P' c o Q' -> TRIPLE P c o Q.
+Proof. move=> HP HQ H. setoid_rewrite ->HP. by setoid_rewrite <-HQ. Qed.
 
 Lemma triple_roc_pre P' P c O Q:
   P |-- P' -> TRIPLE P' c O Q -> TRIPLE P c O Q.
