src/x86/instrrules/in.v
@@ -1,0 +1,16 @@
+(** * IN instruction *)
+Require Import x86.instrrules.core.
+Import x86.instrrules.core.instrruleconfig.
+
+(** Special case for literal port *)
+Require Import x86proved.triple.
+Lemma IN_I_rule (c: BYTE) v w :
+  |-- basic
+      (BYTEregIs AL v) (IN c, AL) (inOP (zeroExtend 8 c) w) (BYTEregIs AL w).
+Proof. instrrule_triple_bazooka. triple.core.triple_by_compute. 
+apply: separateSetRegPiece; eassumption. by rewrite !eq_refl. Qed.
+
+(** We make this rule an instance of the typeclass, and leave
+    unfolding things like [specAtDstSrc] to the getter tactic
+    [get_instrrule_of]. *)
+Instance: forall (c : BYTE), instrrule (IN c, AL) := @IN_I_rule.
